 This theorem ensures that we can switch between summing over ‚Ñï and summing over NonNegInt, a more structured subset of  ‚Ñ§. This transition is useful for formalizing summation equivalences in Lean
```hs
theorem ZTUnilateral_summable_equiv{z : ‚ÑÇ} (x : DiscreteSignal) :
  Summable (fun n : ‚Ñï ‚Ü¶ x n * z ^ (-n : ‚Ñ§)) ‚Üî
  Summable (fun k : NonNegInt ‚Ü¶ x k * z ^ (-k : ‚Ñ§)) := by
    exact Equiv.summable_iff nonNegInt_nat_equiv.symm (
      f := fun (k : NonNegInt) ‚Ü¶ x k * z ^ (-k : ‚Ñ§))
```
This theorem ensures that summability properties hold when switching between standard natural number summations and structured integer sets
```hs
theorem ZTUnilateral_tsum_equiv {z : ‚ÑÇ} (x : DiscreteSignal) :
  (ZTransformUnilateral x) z = (ZTransformUnilateral' x) z := by
    exact Equiv.tsum_eq nonNegInt_nat_equiv.symm (
      fun (k : NonNegInt) ‚Ü¶ x k * z ^ (-k : ‚Ñ§)
    )

theorem indicator_one_mul {Œ± Œ≤ : Type*} [Semiring Œ≤] {A : Set Œ±} (a : Œ±) (f : Œ± ‚Üí Œ≤) :
    A.indicator 1 a * f a = A.indicator (fun a' ‚Ü¶ f a') a := by
      by_cases ha : a ‚àà A
      <;> simp[ha]

theorem zt_summable_causal {z : ‚ÑÇ} {f : DiscreteSignal} :
    (hf : IsCausal f) ‚Üí
    Summable (fun (k : ‚Ñ§) ‚Ü¶ f k * z ^ (-k : ‚Ñ§)) ‚Üî
    Summable (fun (n : ‚Ñï) ‚Ü¶ f n * z ^ (-n : ‚Ñ§)) := by
      intro hf
      apply Iff.intro
      . intro hmp
        simp only[ZTUnilateral_summable_equiv]
        rw[indicator_of_IsCausal_mul hf] at hmp
        exact (summable_subtype_iff_indicator).mpr hmp

      . intro hmpr
        simp only[‚Üêsummable_univ (f := fun k : ‚Ñ§ ‚Ü¶ f k * z ^ (-k : ‚Ñ§))]
        convert Summable.add_compl (s := NegInt) (f := fun k : ‚Ñ§ ‚Ü¶ f k * z ^ (-k : ‚Ñ§)) ?_ ?_

        . exact summable_univ (f := fun k : ‚Ñ§ ‚Ü¶ f k * z ^ (-k : ‚Ñ§))

        . change Summable (fun k : NegInt ‚Ü¶ f k * z ^ (-k : ‚Ñ§))
          refine summable_zero_of_causal (f := fun k ‚Ü¶ f k * z ^ (-k : ‚Ñ§)) ?_
          exact isCausal_of_causal_mul hf

        . change Summable (fun k : ‚ÜëNegInt·∂ú ‚Ü¶ f k * z ^ (-k : ‚Ñ§))
          rw[NegIntComp]
          simp only[‚ÜêZTUnilateral_summable_equiv]
          exact hmpr
```
This theorem shows that if a signal is causal, we can restrict summation to non-negative indices. It justifies the transition from bilateral to unilateral Z-transforms.
```hs
theorem zt_sum_causal {z : ‚ÑÇ} {f : DiscreteSignal} {S : ‚ÑÇ} :
    (hf : IsCausal f) ‚Üí
    HasSum (fun (k : ‚Ñ§) ‚Ü¶ f k * z ^ (-k : ‚Ñ§)) S ‚Üî
    HasSum (fun (n : ‚Ñï) ‚Ü¶ f n * z ^ (-n : ‚Ñ§)) S := by
      intro hf
      apply Iff.intro
      . intro hmp
        simp only[ZTUnilateral_hasSum_equiv]
        rw[indicator_of_IsCausal_mul hf] at hmp
        exact (hasSum_subtype_iff_indicator).mpr hmp

      . intro hmpr
        simp only[‚ÜêhasSum_univ (f := fun k : ‚Ñ§ ‚Ü¶ f k * z ^ (-k : ‚Ñ§))]
        rw[‚Üêneg_nonneg_union]
        convert HasSum.add_disjoint (a := 0) (b := S) (f := fun k : ‚Ñ§ ‚Ü¶ f k * z ^ (-k : ‚Ñ§)) int_neg_nonneg_disjoint ?_ ?_

        . rw[zero_add]

        . change HasSum (fun k : NegInt ‚Ü¶ f k * z ^ (-k : ‚Ñ§)) 0
          refine hasSum_zero_of_causal (f := fun k ‚Ü¶ f k * z ^ (-k : ‚Ñ§)) ?_
          exact isCausal_of_causal_mul hf

        . change HasSum (fun k : NonNegInt ‚Ü¶ f k * z ^ (-k : ‚Ñ§)) S
          simp only[‚ÜêZTUnilateral_hasSum_equiv]
          exact hmpr


theorem zt_sum_unit_step {z : ‚ÑÇ} {f : DiscreteSignal} {S : ‚ÑÇ} :
    HasSum (fun (k : ‚Ñ§) ‚Ü¶ u k * f k * z ^ (-k : ‚Ñ§)) S ‚Üî
    HasSum (fun (n : ‚Ñï) ‚Ü¶ f n * z ^ (-n : ‚Ñ§)) S := by

      convert zt_sum_causal (causal_of_unit_step_mul f) with n
      simp[u]
```
The preceding sub-theorems systematically reduce summation complexity and enforce causality in formal Z-transform proofs. They ensure that we only consider non-negative indices, enabling a rigorous transition from bilateral to unilateral Z-transforms. With all that done, we can finaly prove the unit step Z-transformation 
```hs
theorem zt_unit_step {z : ‚ÑÇ} (h_roc : ‚Äñz‚Äñ > 1) : HasZTransform u (fun z ‚Ü¶ (1 / (1 - z‚Åª¬π))) z := by
  rw[HasZTransform]

  suffices ‚àÄ k, u k * z ^ (-k) = u k * 1 * z ^ (-k) by
    simp only [this]

    refine' zt_sum_unit_step.mpr _
    simp
    simp only[‚Üêinv_pow]

    refine' hasSum_geometric_of_norm_lt_one _
    rw[norm_inv, inv_lt_comm‚ÇÄ] <;> linarith

  simp





theorem ZTransformToDTFT : ‚àÄ x : DiscreteSignal, (fun œâ : ‚Ñù => ùì© x (Complex.exp (j * œâ))) = ùìï_d x := by
  intro x
  ext œâ
  simp
  apply tsum_congr
  intro k
  calc
    x k * (Complex.exp (j * ‚Üëœâ) ^ k)‚Åª¬π
      = x k * (Complex.exp (j * ‚Üëœâ * ‚Üëk))‚Åª¬π := by rw [‚Üê Complex.exp_int_mul (j * ‚Üëœâ) k]; ring_nf
    _ = x k * Complex.exp (-(j * ‚Üëœâ * ‚Üëk)) := by rw [‚ÜêComplex.exp_neg (j * ‚Üëœâ * ‚Üëk)]



theorem zt_mul_left (z : ‚ÑÇ) (f‚ÇÅ : DiscreteSignal) (F‚ÇÅ : ‚ÑÇ ‚Üí ‚ÑÇ) (a : ‚ÑÇ)
(hz‚ÇÅ : HasZTransform f‚ÇÅ F‚ÇÅ z) :
  HasZTransform (fun k => a * f‚ÇÅ k) (fun z => a * F‚ÇÅ z) z := by
  unfold HasZTransform
  change HasSum (fun k ‚Ü¶ a * f‚ÇÅ k * z ^ (-k)) (( a * F‚ÇÅ z))
  simp only[mul_assoc]
  apply HasSum.mul_left a hz‚ÇÅ

theorem zt_mul_right (z : ‚ÑÇ) (f‚ÇÅ : DiscreteSignal) (F‚ÇÅ : ‚ÑÇ ‚Üí ‚ÑÇ) (a : ‚ÑÇ)
(hz‚ÇÅ : HasZTransform f‚ÇÅ F‚ÇÅ z) :
  HasZTransform (fun k => f‚ÇÅ k * a) (fun z => F‚ÇÅ z * a) z := by
  unfold HasZTransform
  change HasSum (fun k ‚Ü¶  f‚ÇÅ  k  * a * z ^ (-k) ) ((F‚ÇÅ z * a))
  have: (Œª k ‚Ü¶ f‚ÇÅ  k  * a * z ^ (-k)) = (Œª k ‚Ü¶ f‚ÇÅ  k   * z ^ (-k) * a ):= by
    ext k
    ring_nf
  -- ‚ä¢ HasSum (fun k ‚Ü¶ f‚ÇÅ k * a * z ^ (-k)) (F‚ÇÅ z * a)
  simp only[this]
  apply HasSum.mul_right a hz‚ÇÅ

theorem zt_add (z : ‚ÑÇ) (f‚ÇÅ f‚ÇÇ : DiscreteSignal) (F‚ÇÅ F‚ÇÇ : ‚ÑÇ ‚Üí ‚ÑÇ) (hz‚ÇÅ : HasZTransform f‚ÇÅ F‚ÇÅ z)  (hz‚ÇÇ: HasZTransform f‚ÇÇ F‚ÇÇ z) :
   HasZTransform (fun k => f‚ÇÅ k + f‚ÇÇ k) (fun z => F‚ÇÅ z + F‚ÇÇ z) z := by
    unfold HasZTransform -- (fun k ‚Ü¶ (fun k ‚Ü¶ f‚ÇÅ k + f‚ÇÇ k) k * z ^ (-k)) ((fun z ‚Ü¶ F‚ÇÅ z + F‚ÇÇ z) z)
    change HasSum (fun k ‚Ü¶ (f‚ÇÅ k + f‚ÇÇ k) * z ^ (-k)) ( F‚ÇÅ z + F‚ÇÇ z)
    have :  (fun k ‚Ü¶ (f‚ÇÅ k + f‚ÇÇ k) * z ^ (-k)) = (fun k ‚Ü¶(f‚ÇÅ k) * z ^ (-k) + (f‚ÇÇ k) * z ^ (-k)) := by
      ext k
      ring_nf
    simp only[this]
    apply HasSum.add  hz‚ÇÅ hz‚ÇÇ
```
